theories/backends/ASTBackend.v
@@ -1,12 +1,12 @@
 From ExtLib.Structures Require Import Monad.
 From MetaRocq.Utils Require Import utils.
 From MetaRocq.Utils Require Import bytestring.
-From CertiCoq Require Import Compiler.pipeline.
-From CertiCoq Require Import Common.Pipeline_utils.
+From CertiRocq Require Import Compiler.pipeline.
+From CertiRocq Require Import Common.Pipeline_utils.
 From Peregrine Require Import Config.
 From Peregrine Require Import Utils.
 From Peregrine Require Import PAst.
-From Peregrine Require Import CertiCoqBackend.
+From Peregrine Require Import CertiRocqBackend.
 From Peregrine Require SerializePAst.
 From Peregrine Require SerializeLambdaBoxMut.
 From Peregrine Require SerializeLambdaBoxLocal.
@@ -53,7 +53,7 @@ Definition extract_typed_ast (p : ExAst.global_env)
   Ok (SerializePAst.string_of_PAst (Typed p None)).
 
 Definition extract_mut_ast (remaps : constant_remappings)
-                           (opts : certicoq_config)
+                           (opts : certirocq_config)
                            (p : EAst.program)
                            : result string string :=
   let config := mk_opts opts in
@@ -67,7 +67,7 @@ Definition extract_mut_ast (remaps : constant_remappings)
   end.
 
 Definition extract_local_ast (remaps : constant_remappings)
-                             (opts : certicoq_config)
+                             (opts : certirocq_config)
                              (p : EAst.program)
                             : result string string :=
   let config := mk_opts opts in
@@ -82,7 +82,7 @@ Definition extract_local_ast (remaps : constant_remappings)
 
 
 Definition extract_anf_ast (remaps : constant_remappings)
-                           (opts : certicoq_config)
+                           (opts : certirocq_config)
                            (p : EAst.program)
                            : result string string :=
   let config := mk_opts opts in
@@ -97,7 +97,7 @@ Definition extract_anf_ast (remaps : constant_remappings)
 
 
 Definition extract_anfc_ast (remaps : constant_remappings)
-                            (opts : certicoq_config)
+                            (opts : certirocq_config)
                             (p : EAst.program)
                             : result string string :=
   let config := mk_opts opts in
